StrataTest/DL/Lambda/LExprEvalTests.lean
@@ -4,6 +4,7 @@
   SPDX-License-Identifier: Apache-2.0 OR MIT
 -/
 
+import Strata.DL.Lambda.Semantics
 import Strata.DL.Lambda.LExprEval
 
 ---------------------------------------------------------------------
@@ -19,54 +20,188 @@ section EvalTest
 open LTy.Syntax LExpr.SyntaxMono
 open Std (ToFormat Format format)
 
+/-
+Each test is a pair of
+1. Lambda.LExpr.eval invocation, and
+2. Its equivalent Lambda.LExpr.Step version.
+-/
+
+-- A helper tactic for proving 'isCanonicalValue e = b'.
+macro "discharge_isCanonicalValue": tactic => `(tactic|
+    conv =>
+      lhs; reduce; unfold isCanonicalValue; reduce; unfold isCanonicalValue
+  )
+-- Take a small step.
+macro "take_step": tactic => `(tactic |
+    (conv => lhs; reduce) <;> apply StepStar.step
+  )
+-- Finish taking small steps!
+macro "take_refl": tactic => `(tactic |
+    (conv => lhs; reduce) <;> apply StepStar.refl
+  )
+-- Do beta reduction.
+macro "reduce_beta": tactic => `(tactic |
+    apply Step.beta <;> discharge_isCanonicalValue
+  )
+-- A helper tactic to exhibit an instance of Metadata (which is Unit)
+macro "inhabited_metadata": tactic => `(tactic |
+    solve | (simp; apply ())
+  )
+
 private abbrev TestParams : LExprParams := ⟨Unit, Unit⟩
 
 private instance : Coe String TestParams.Identifier where
   coe s := Identifier.mk s ()
 
-/-- info: (λ (if (%0 == #1) then #10 else (_minit %0))) -/
-#guard_msgs in
-#eval format $ Lambda.LExpr.eval (TBase:=TestParams) 100
-                  {Lambda.LState.init with state :=
-                      [[("m", (mty[int → int], esM[_minit]))]] }
-        esM[λ (if (%0 == #1) then #10 else (m %0))]
 
-/-- info: #42 -/
-#guard_msgs in
-#eval format $ LExpr.eval (TBase:=TestParams) 100
-                          { LState.init with state := [[("x", (mty[int], esM[#32]))]] }
-                          esM[((λ (if (%0 == #23) then #17 else #42)) (x : int))]
+/- Test cases -/
 
-/-- info: (f #true) -/
-#guard_msgs in
-#eval format $ LExpr.eval (TBase:=TestParams) 10 ∅ esM[(f #true)]
+structure TestCase where
+  -- Input state
+  σ: LState TestParams
+  -- Input expression
+  e: LExpr (TestParams.mono)
+  -- Reduced output
+  e_out: LExpr (TestParams.mono)
 
-/-- info: (minit #24) -/
-#guard_msgs in
-#eval format $ LExpr.eval (TBase:=TestParams) 100
-                    { LState.init with state :=
-                        [[("m", (none, esM[(λ (minit %0))]))], -- most recent scope
-                         [("m", (none, (.intConst () 12)))]] }
-                    esM[((λ (if (%0 == #23) then #17 else (m %0)) #24))]
+def check (t:TestCase) (n:=100) := (Lambda.LExpr.eval n t.σ t.e) == t.e_out
 
-/-- info: (minit #24) -/
-#guard_msgs in
-#eval format $ LExpr.eval (TBase:=TestParams) 100
-                    { LState.init with state := [[("m", (none, esM[minit]))]] }
-                    esM[((λ (if (%0 == #23) then #17 else (m %0))) #24)]
+/-- The two kinds of propositions we would like to test! -/
+abbrev steps_well (t:TestCase):Prop :=
+  Lambda.StepStar (Tbase:=TestParams)
+    t.σ.config.factory (Scopes.toEnv t.σ.state) t.e t.e_out
 
-/-- info: x -/
+abbrev stuck (t:TestCase):Prop :=
+  ∀ eres, ¬ Lambda.Step (Tbase:=TestParams)
+    t.σ.config.factory (Scopes.toEnv t.σ.state) t.e eres
+
+
+-------------------------------- Tests ------------------------------
+
+def test1 := TestCase.mk
+  ({Lambda.LState.init with state := [[("m", (mty[int → int], esM[_minit]))]] })
+  (esM[λ (if (%0 == #1) then #10 else (m %0))])
+  (esM[λ (if (%0 == #1) then #10 else (_minit %0))])
+
+/-- info: true -/
 #guard_msgs in
-#eval format $ LExpr.eval (TBase:=TestParams) 10 ∅ esM[if #true then x else y]
+#eval (check test1)
+
+-- Small step stucks because abstraction is a value.
+example: stuck test1 := by
+  intros e H
+  contradiction
+
+
+def test2 := TestCase.mk
+  { LState.init with state := [[("x", (mty[int], esM[#32]))]] }
+  esM[((λ (if (%0 == #23) then #17 else #42)) (x : int))]
+  esM[#42]
+
+/-- info: true -/
+#guard_msgs in
+#eval (check test2)
+
+example: steps_well test2 := by
+  unfold steps_well Scopes.toEnv test2
+  take_step; apply Step.reduce_2 <;> try inhabited_metadata
+  · discharge_isCanonicalValue
+  · repeat constructor
+  take_step; reduce_beta
+  take_step; constructor <;> try inhabited_metadata
+  · apply Step.eq_reduce <;> try discharge_isCanonicalValue
+    · inhabited_metadata
+  take_step; apply Step.ite_reduce_else
+  apply StepStar.refl
+
+
+def test3 := TestCase.mk
+  ∅
+  esM[(f #true)]
+  esM[(f #true)]
+
+/-- info: true -/
+#guard_msgs in
+#eval check test3
+
+example: stuck test3 := by
+  intros e H
+  contradiction
+
+
+def test4 := TestCase.mk
+  { LState.init with state :=
+      [[("m", (none, esM[(λ (minit %0))]))], -- most recent scope
+      [("m", (none, (.intConst () 12)))]] }
+  esM[((λ (if (%0 == #23) then #17 else (m %0)) #24))]
+  esM[(minit #24)]
+
+/-- info: true -/
+#guard_msgs in
+#eval check test4
+
+example: steps_well test4 := by
+  unfold steps_well Scopes.toEnv test4
+  take_step; reduce_beta
+  take_step; apply Step.ite_reduce_cond <;> try inhabited_metadata
+  · apply Step.eq_reduce <;> try discharge_isCanonicalValue
+    · inhabited_metadata
+  take_step; apply Step.ite_reduce_else
+  take_step; apply Step.reduce_1; inhabited_metadata; apply Step.expand_fvar; rfl
+  take_step; reduce_beta
+  take_refl
+
+
+def test5 := TestCase.mk
+  { LState.init with state := [[("m", (none, esM[minit]))]] }
+  esM[((λ (if (%0 == #23) then #17 else (m %0))) #24)]
+  esM[(minit #24)]
+
+/-- info: true -/
+#guard_msgs in
+#eval check test5
+
+example: steps_well test5 := by
+  unfold steps_well Scopes.toEnv test5
+  take_step; reduce_beta
+  take_step; apply Step.ite_reduce_cond; inhabited_metadata
+  · apply Step.eq_reduce <;> try discharge_isCanonicalValue
+    · inhabited_metadata
+  take_step; apply Step.ite_reduce_else
+  take_step; apply Step.reduce_1; inhabited_metadata; apply Step.expand_fvar; rfl
+  take_refl
+
+
+def test6 := TestCase.mk
+  ∅
+  esM[if #true then x else y]
+  esM[x]
+
+/-- info: true -/
+#guard_msgs in
+#eval check test6
+
+example: steps_well test6 := by
+  unfold steps_well Scopes.toEnv test6
+  take_step
+  · constructor
+  take_refl
+
 
 -- Ill-formed `abs` is returned as-is in this Curry style...
-/-- info: (λ %1) -/
-#guard_msgs in
-#eval format $ LExpr.eval (TBase:=TestParams) 10 ∅ esM[(λ %1)]
+def test7 := TestCase.mk
+  ∅
+  esM[(λ %1)]
+  esM[(λ %1)]
 
-/-- info: ((λ %1) #true) -/
+/-- info: true -/
 #guard_msgs in
-#eval format $ LExpr.eval (TBase:=TestParams) 0 ∅ (.app () (.abs () .none (.bvar () 1)) (LExpr.true ()))
+#eval check test7
+
+example: stuck test7 := by
+  intros e H
+  contradiction
+
 
 /- Tests for evaluation of BuiltInFunctions. -/
 
@@ -120,82 +255,380 @@ private def testState : LState TestParams :=
   | .error e => panic s!"{e}"
   | .ok ok => ok
 
-/-- info: #50 -/
-#guard_msgs in
-#eval format $ LExpr.eval (TBase:=TestParams) 10 testState esM[((~IntAddAlias #20) #30)]
 
-/-- info: ((~Int.Add #20) x) -/
-#guard_msgs in
-#eval format $ LExpr.eval (TBase:=TestParams) 10 testState esM[((~IntAddAlias #20) x)]
+def test8 := TestCase.mk
+  testState
+  esM[((~IntAddAlias #20) #30)]
+  esM[(#50)]
 
-/-- info: ((~Int.Add ((~Int.Add #5) #100)) x) -/
+/-- info: true -/
 #guard_msgs in
-#eval format $ LExpr.eval (TBase:=TestParams) 10 LState.init esM[(( ((λλ (~Int.Add %1) %0)) ((λ ((~Int.Add %0) #100)) #5)) x)]
+#eval check test8
 
-/-- info: #50 -/
-#guard_msgs in
-#eval format $ LExpr.eval (TBase:=TestParams) 10 testState esM[((~Int.Add #20) #30)]
+example: steps_well test8 := by
+  unfold steps_well Scopes.toEnv test8
+  take_step; apply Step.expand_fn <;> discharge_isCanonicalValue
+  take_step; apply Step.eval_fn <;> try discharge_isCanonicalValue
+  · inhabited_metadata
+  take_refl
 
-/-- info: ((~Int.Add #105) x) -/
-#guard_msgs in
-#eval format $ LExpr.eval (TBase:=TestParams) 10 testState esM[((((λλ (~Int.Add %1) %0)) ((λ ((~Int.Add %0) #100)) #5)) x)]
 
-/-- info: ((#f #20) #-5) -/
-#guard_msgs in
-#eval format $ LExpr.eval (TBase:=TestParams) 10 testState esM[( ((λλ (#f %1) %0) #20) ((λ (~Int.Neg %0)) #5))]
+def test9 := TestCase.mk
+  testState
+  esM[((~IntAddAlias #20) x)]
+  esM[((~Int.Add #20) x)]
 
-/-- info: ((~Int.Add #20) (~Int.Neg x)) -/
+/-- info: true -/
 #guard_msgs in
-#eval format $ LExpr.eval (TBase:=TestParams) 10 testState esM[( ((λλ (~Int.Add %1) %0) #20) ((λ (~Int.Neg %0)) x))]
+#eval check test9
 
-/-- info: ((~Int.Add #20) (~Int.Neg x)) -/
-#guard_msgs in
-#eval format $ LExpr.eval (TBase:=TestParams) 10 testState esM[((~Int.Add #20) (~Int.Neg x))]
+-- Note: this case diverges from concrete evaluator, because 'x' is not a
+-- canonical value! Small step reduces only when the arguments are values,
+-- to avoid nondeterminism in the small-step semantics (unless this becomes
+-- explicitly allowed in the future).
+example: stuck test9 := by
+  intro e H; cases H
+  case reduce_2 => contradiction
+  case reduce_1 => contradiction
+  case expand_fn =>
+    rename_i Hlfunc Hfv
+    conv at Hlfunc => lhs; reduce
+    cases Hlfunc
+    rename_i Hconst Htmp
+    conv at Hconst => lhs; reduce; unfold isCanonicalValue; reduce
+    contradiction
+  case eval_fn =>
+    rename_i Hlfunc
+    conv at Hlfunc => lhs; reduce
+    cases Hlfunc
+    rename_i Hconst Htmp
+    conv at Hconst => lhs; reduce; unfold isCanonicalValue; reduce
+    contradiction
 
-/-- info: ((~Int.Add x) #-30) -/
-#guard_msgs in
-#eval format $ LExpr.eval (TBase:=TestParams) 10 testState esM[((~Int.Add x) (~Int.Neg #30))]
 
-/-- info: #50 -/
+-- A sanity check that confirms the parse tree of λλ x y
+/-- info: true -/
 #guard_msgs in
-#eval format $ LExpr.eval (TBase:=TestParams) 10 testState esM[((λ %0) ((~Int.Add #20) #30))]
+#eval esM[(λλ (~Int.Add %1) %0)] = esM[((λ(λ (~Int.Add %1))) %0)]
 
-/-- info: #100 -/
-#guard_msgs in
-#eval format $ LExpr.eval (TBase:=TestParams) 10 testState esM[((~Int.Div #300) ((~Int.Add #2) #1))]
 
-/-- info: #0 -/
-#guard_msgs in
-#eval format $ LExpr.eval (TBase:=TestParams) 10 testState esM[((~Int.Add #3) (~Int.Neg #3))]
+def test10 := TestCase.mk
+  LState.init
+  esM[(( ((λ(λ ((~Int.Add %1) %0)))) ((λ ((~Int.Add %0) #100)) #5)) x)]
+  esM[((~Int.Add ((~Int.Add #5) #100)) x)]
 
-/-- info: #0 -/
+/-- info: true -/
 #guard_msgs in
-#eval format $ LExpr.eval (TBase:=TestParams) 10 testState esM[((~Int.Add (~Int.Neg #3)) #3)]
+#eval check test10
 
-/-- info: ((~Int.Div #300) #0) -/
-#guard_msgs in
-#eval format $ LExpr.eval (TBase:=TestParams) 10 testState esM[((~Int.Div #300) ((~Int.Add #3) (~Int.Neg #3)))]
+-- The small step semantics of this example will stuck in the middle because
+-- 'Int.Add %0 100' cannot be evaluated because the definition of Int.Add is
+-- not available in LState.init .
 
-/-- info: ((~Int.Div x) #3) -/
-#guard_msgs in
-#eval format $ LExpr.eval (TBase:=TestParams) 10 testState esM[((~Int.Div x) ((~Int.Add #2) #1))]
 
-/-- info: ((~Int.Le #100) x) -/
-#guard_msgs in
-#eval format $ LExpr.eval (TBase:=TestParams) 200 testState
-                esM[((~Int.Le ((~Int.Div #300) ((~Int.Add #2) #1))) x)]
+def test11 := TestCase.mk
+  testState
+  esM[((~Int.Add #20) #30)]
+  esM[#50]
 
-/--
-info: ((~Int.Le ((~Int.Div #300) ((~Int.Add #2) y))) x)
--/
+/-- info: true -/
 #guard_msgs in
-#eval format $ LExpr.eval (TBase:=TestParams) 200 testState
-                esM[((~Int.Le ((~Int.Div #300) ((~Int.Add #2) y))) x)]
+#eval check test11
 
-/-- info: ((~Int.Div x) x) -/
+example: steps_well test11 := by
+  unfold steps_well Scopes.toEnv test11
+  take_step; apply Step.eval_fn <;> try discharge_isCanonicalValue
+  · inhabited_metadata
+  take_refl
+
+
+def test12 := TestCase.mk
+  testState
+  esM[((((λ(λ (~Int.Add %1) %0))) ((λ ((~Int.Add %0) #100)) #5)) x)]
+  esM[((~Int.Add #105) x)]
+
+/-- info: true -/
 #guard_msgs in
-#eval format $ LExpr.eval (TBase:=TestParams) 200 testState
-                esM[((~Int.Div x) x)]
+#eval check test12
+
+example: steps_well test12 := by
+  unfold steps_well Scopes.toEnv test12
+  take_step; apply Step.reduce_1; inhabited_metadata; apply Step.reduce_2
+  · inhabited_metadata;
+  · discharge_isCanonicalValue
+  · reduce_beta
+  take_step; apply Step.reduce_1; inhabited_metadata; apply Step.reduce_2;
+  · inhabited_metadata;
+  · discharge_isCanonicalValue
+  · apply Step.eval_fn <;> try discharge_isCanonicalValue
+    · inhabited_metadata
+  take_step; apply Step.reduce_1; inhabited_metadata; reduce_beta
+  take_step; apply Step.reduce_1; inhabited_metadata; reduce_beta
+  take_refl
+
+/-- info: false -/
+#guard_msgs in
+#eval LExpr.isCanonicalValue testState.config.factory esM[((~Int.Add #100) #200)]
+
+/-- info: true -/
+#guard_msgs in
+#eval LExpr.isCanonicalValue testState.config.factory esM[(~Int.Add #100)]
+
+
+def test13 := TestCase.mk
+  testState
+  esM[( ((λ(λ (#f %1) %0) #20)) ((λ (~Int.Neg %0)) #5))]
+  esM[((#f #20) #-5)]
+
+/-- info: true -/
+#guard_msgs in
+#eval check test13
+
+-- The small step semantics of this example will stuck in the middle because
+-- '(#f 20) e' cannot be evaluated because the definition of #f is
+-- not available.
+
+
+def test14 := TestCase.mk
+  testState
+  esM[( ((λ(λ (~Int.Add %1) %0)) #20) ((λ (~Int.Neg %0)) x))]
+  esM[((~Int.Add #20) (~Int.Neg x))]
+
+/-- info: true -/
+#guard_msgs in
+#eval check test14
+
+-- The result stops at (.. ((λ (~Int.Neg %0)) x)) because definition of
+-- x is not available.
+example: steps_well { test14 with e_out := esM[((~Int.Add #20) ((λ (~Int.Neg %0)) x))] }
+  := by
+  unfold steps_well Scopes.toEnv test14
+  take_step; apply Step.reduce_1; inhabited_metadata; reduce_beta
+  take_step; apply Step.reduce_1; inhabited_metadata; reduce_beta
+  take_refl
+
+
+def test15 := TestCase.mk
+  testState
+  esM[((~Int.Add #20) (~Int.Neg x))]
+  esM[((~Int.Add #20) (~Int.Neg x))]
+
+/-- info: true -/
+#guard_msgs in
+#eval check test15
+
+example: stuck test15 := by
+  intros e H
+  cases H <;> try contradiction
+  case reduce_2 =>
+    rename_i a
+    cases a <;> try contradiction
+    · rename_i a a2 _
+      cases a2; cases a
+    · rename_i a a2 a3
+      cases a3
+      conv at a => lhs ; reduce; unfold isCanonicalValue; reduce
+      contradiction
+  case expand_fn =>
+    rename_i a a2 a3
+    cases a2
+    contradiction
+  case eval_fn =>
+    rename_i a a2 a3
+    cases a3
+    conv at a => lhs ; reduce; unfold isCanonicalValue; reduce
+    contradiction
+
+
+def test16 := TestCase.mk
+  testState
+  esM[((~Int.Add x) (~Int.Neg #30))]
+  esM[((~Int.Add x) #-30)]
+
+/-- info: true -/
+#guard_msgs in
+#eval check test16
+
+-- test16 stucks because '~Int.Add x' isn't canonical value.
+example: stuck test16 := by
+  intros e H
+  cases H <;> try contradiction
+  case reduce_2 =>
+    rename_i a a2
+    conv at a => lhs; unfold isCanonicalValue; reduce; unfold isCanonicalValue; reduce
+    contradiction
+  case expand_fn =>
+    rename_i a a2 a3
+    cases a2
+    contradiction
+  case eval_fn =>
+    rename_i a a2 a3
+    cases a3
+    conv at a => lhs ; reduce; unfold isCanonicalValue; reduce
+    contradiction
+
+
+def test17 := TestCase.mk
+  testState
+  esM[((λ %0) ((~Int.Add #20) #30))]
+  esM[(#50)]
+
+/-- info: true -/
+#guard_msgs in
+#eval check test17
+
+example: steps_well test17 := by
+  unfold steps_well Scopes.toEnv test17
+  take_step; apply Step.reduce_2
+  · inhabited_metadata
+  · discharge_isCanonicalValue
+  · apply Step.eval_fn <;> try discharge_isCanonicalValue
+    · inhabited_metadata
+  take_step; reduce_beta
+  take_refl
+
+
+def test18 := TestCase.mk
+  testState
+  esM[((~Int.Div #300) ((~Int.Add #2) #1))]
+  esM[(#100)]
+
+/-- info: true -/
+#guard_msgs in
+#eval check test18
+
+example: steps_well test18 := by
+  unfold steps_well Scopes.toEnv test18
+  take_step; apply Step.reduce_2
+  · inhabited_metadata
+  · discharge_isCanonicalValue
+  · apply Step.eval_fn <;> try discharge_isCanonicalValue
+    · inhabited_metadata
+  take_step; apply Step.eval_fn <;> try discharge_isCanonicalValue
+  · inhabited_metadata
+  take_refl
+
+
+def test19 := TestCase.mk
+  testState
+  esM[((~Int.Add #3) (~Int.Neg #3))]
+  esM[(#0)]
+
+/-- info: true -/
+#guard_msgs in
+#eval check test19
+
+example: steps_well test19 := by
+  unfold steps_well Scopes.toEnv test19
+  take_step
+  · apply Step.reduce_2
+    · inhabited_metadata
+    · discharge_isCanonicalValue
+    · apply Step.eval_fn <;> try discharge_isCanonicalValue
+      · inhabited_metadata
+  take_step
+  · apply Step.eval_fn <;> try rfl
+    · inhabited_metadata
+    · conv => lhs; reduce; unfold isCanonicalValue; reduce
+  take_refl
+
+
+def test20 := TestCase.mk
+  testState
+  esM[((~Int.Add (~Int.Neg #3)) #3)]
+  esM[(#0)]
+
+/-- info: true -/
+#guard_msgs in
+#eval check test20
+
+example: steps_well test20 := by
+  unfold steps_well Scopes.toEnv test20
+  take_step; apply Step.reduce_1
+  · inhabited_metadata
+  · apply Step.reduce_2
+    · inhabited_metadata
+    · discharge_isCanonicalValue
+    · apply Step.eval_fn <;> try discharge_isCanonicalValue
+      · inhabited_metadata
+  take_step; apply Step.eval_fn <;> try discharge_isCanonicalValue
+  · inhabited_metadata
+  take_refl
+
+
+def test21 := TestCase.mk
+  testState
+  esM[((~Int.Div #300) ((~Int.Add #3) (~Int.Neg #3)))]
+  esM[((~Int.Div #300) #0)]
+
+/-- info: true -/
+#guard_msgs in
+#eval check test21
+
+example: steps_well test21 := by
+  unfold steps_well Scopes.toEnv test21
+  take_step; apply Step.reduce_2
+  · inhabited_metadata
+  · discharge_isCanonicalValue
+  · apply Step.reduce_2
+    · inhabited_metadata
+    · discharge_isCanonicalValue
+    · apply Step.eval_fn <;> try discharge_isCanonicalValue
+      · inhabited_metadata
+  take_step; apply Step.reduce_2
+  · inhabited_metadata
+  · discharge_isCanonicalValue
+  · apply Step.eval_fn <;> try discharge_isCanonicalValue
+    · inhabited_metadata
+  take_refl
+
+
+def test22 := TestCase.mk
+  testState
+  esM[((~Int.Div x) ((~Int.Add #2) #1))]
+  esM[((~Int.Div x) #3)]
+
+/-- info: true -/
+#guard_msgs in
+#eval check test22
+
+-- TODO: steps_well proof of test22
+
+
+def test23 := TestCase.mk
+  testState
+  esM[((~Int.Le ((~Int.Div #300) ((~Int.Add #2) #1))) x)]
+  esM[((~Int.Le #100) x)]
+
+/-- info: true -/
+#guard_msgs in
+#eval check test23
+
+-- TODO: steps_well proof of test23
+
+
+def test24 := TestCase.mk
+  testState
+  esM[((~Int.Le ((~Int.Div #300) ((~Int.Add #2) y))) x)]
+  esM[((~Int.Le ((~Int.Div #300) ((~Int.Add #2) y))) x)]
+
+/-- info: true -/
+#guard_msgs in
+#eval check test24
+
+-- TODO: stuck proof of test24
+
+
+def test25 := TestCase.mk
+  testState
+  esM[((~Int.Div x) x)]
+  esM[((~Int.Div x) x) ]
+
+/-- info: true -/
+#guard_msgs in
+#eval check test25
+
+-- TODO: stuck proof of test25
 
 
 end EvalTest
